Removed Var type. Rewrote some functions.

Loop/Basic.lean
@@ -10,29 +10,25 @@ Loop-computable is the same as primitive recursive.
 
 namespace Loop
 
-structure Var where
-  X : Nat
-
-abbrev X₀ : Var := ⟨0⟩
 
 inductive Instruction where
-  | clear_var : Var → Instruction
-  | increment_var : Var → Instruction
-  | loop_var : Var → List Instruction → Instruction
+  | clear_var : Nat → Instruction
+  | increment_var : Nat → Instruction
+  | loop_var : Nat → List Instruction → Instruction
 open Instruction
 
 
-notation "CLEAR X " n:68 => clear_var ⟨n⟩
-notation "INC X " n:68 => increment_var ⟨n⟩
-notation "LOOP X " n " DO " ls:68 => loop_var ⟨n⟩ ls
+notation "CLEAR X " n:68 => clear_var n
+notation "INC X " n:68 => increment_var n
+notation "LOOP X " n " DO " ls:68 => loop_var n ls
 
 abbrev END : List Instruction := []
 
 
-/- A Loop program is a list of instructions. -/
+-- /- A Loop program is a list of instructions. -/
 def Program := List Instruction
 
-example : Program := END
+-- example : Program := END
 
 def example_1 : Program :=
   LOOP X 1 DO (
@@ -45,24 +41,23 @@ def example_1 : Program :=
 def VarState := List Nat
 
 
-def Var.value_at : VarState → Var → Nat
-  | xs, ⟨n⟩ => xs.getD n 0
+def value_at : VarState → Nat → Nat
+  | xs, n => xs.getD n 0
 
-example : Var.value_at [3, 1, 5] ⟨2⟩ = 5 := rfl
-example : Var.value_at [3, 1, 5] ⟨7⟩ = 0 := rfl
+example : value_at [3, 1, 5] 2 = 5 := rfl
+example : value_at [3, 1, 5] 7 = 0 := rfl
 
-def Var.clear_value : VarState → Var → VarState
-  | xs, ⟨n⟩ => xs.set n 0
+def clear_value : VarState → Nat → VarState
+  | xs, n => xs.set n 0
 
-example : Var.clear_value [3, 1, 5] ⟨2⟩ = [3, 1, 0] := rfl
+example : clear_value [3, 1, 5] 2 = [3, 1, 0] := rfl
 
-def Var.inc_value : VarState → Var → VarState
-  | xs, v@⟨n⟩ => xs.set n (v.value_at xs + 1)
+def inc_value : VarState → Nat → VarState
+  | xs, n => xs.set n (value_at xs n + 1)
 
-example : Var.inc_value [3, 1, 5] ⟨2⟩ = [3, 1, 6] := by rfl
+example : inc_value [3, 1, 5] 2 = [3, 1, 6] := by rfl
 
-def init_state (v : Mathlib.Vector Nat n) : VarState := match v with
-  | ⟨xs, _⟩ => 0 :: xs
+def init_state (v : Mathlib.Vector Nat n) : VarState := 0 :: v.toList
 
 mutual
   def lines_of_code : Program → Nat
@@ -76,43 +71,51 @@ mutual
     | _ => 1
 end
 
+attribute [local simp] lines_of_code lines_of_code_instruction
+
 example : lines_of_code example_1 = 3 := rfl
 
-mutual
-    def loop_n_times : Nat → VarState  → Program → VarState
-      | 0, xs, _ => xs
-      | n + 1, xs, p => loop_n_times n (execution_from_state xs p) p
-    termination_by n _ p => (lines_of_code p, n)
+def execution_from_state (xs : VarState) (p : Program) : VarState :=
+  let rec loop_n_times : Nat → VarState → Program → VarState
+  | 0, xs, _ => xs
+  | n + 1, xs, p => loop_n_times n (execution_from_state xs p) p
+  termination_by n _ p => (lines_of_code p, n)
 
-    def execution_from_state (xs : VarState) : Program → VarState
-    | [] => xs
-    | .clear_var v      :: tail =>
-      have : lines_of_code tail < lines_of_code (clear_var v :: tail) := by
-        simp [lines_of_code]
-      execution_from_state (v.clear_value xs) tail
-    | .increment_var v  :: tail =>
-      have : lines_of_code tail < lines_of_code (increment_var v :: tail) := by
-        simp [lines_of_code]
-      execution_from_state (v.inc_value xs) tail
-    | .loop_var v inner :: tail =>
-      have : lines_of_code inner < lines_of_code (loop_var v inner :: tail) := by
-        simp_arith [lines_of_code, lines_of_code_instruction]
-      have : lines_of_code tail < lines_of_code (loop_var v inner :: tail) := by
-        simp_arith [lines_of_code, lines_of_code_instruction]
-      execution_from_state (loop_n_times (v.value_at xs) xs inner) tail
-    termination_by p => (lines_of_code p, 0)
-end
+  match p with
+  | [] => xs
+  | .clear_var k      :: tail =>
+    execution_from_state (clear_value xs k) tail
+  | .increment_var k  :: tail =>
+    execution_from_state (inc_value xs k) tail
+  | .loop_var k inner :: tail =>
+    execution_from_state (loop_n_times (value_at xs k) xs inner) tail
+termination_by (lines_of_code p, 0)
+open execution_from_state.loop_n_times
+
 
 def nary_program_function (p : Program) (n : Nat) (v : Mathlib.Vector Nat n) : Nat :=
-  X₀.value_at (execution_from_state (init_state v) p)
+  value_at (execution_from_state (init_state v) p) 0
 
 notation "⟦ " p " ⟧^(" n ") " => nary_program_function p n
 
 example : ⟦ example_1 ⟧^(2) ⟨[11, 11], rfl⟩ = 121 := by
-  simp [nary_program_function, init_state, example_1, execution_from_state, loop_n_times, Var.value_at, Var.inc_value, Var.clear_value]
+  simp [nary_program_function, init_state, example_1, execution_from_state, loop_n_times, value_at, inc_value, clear_value]
 
 
 def loop_computable (f : Mathlib.Vector Nat n → Nat) : Prop :=
   ∃ p : Program, ⟦ p ⟧^(n) = f
 
--------
+-- -- -------
+-- def highest_var : Program → Nat
+--   | [] => 0
+--   | clear_var k :: tail =>
+--     have : lines_of_code tail < lines_of_code (clear_var k :: tail) := by simp
+--     max k (highest_var tail)
+--   | increment_var k :: tail =>
+--     have : lines_of_code tail < lines_of_code (increment_var k :: tail) := by simp
+--     max k (highest_var tail)
+--   | loop_var k inner :: tail =>
+--     have : lines_of_code inner < lines_of_code (loop_var k inner :: tail) := by simp_arith
+--     have : lines_of_code tail < lines_of_code (loop_var k inner :: tail) := by simp_arith
+--     max k (max (highest_var inner) (highest_var tail))
+-- termination_by p => lines_of_code p
